---
layout: post
name: Fair Resource Distribution Algorithm
tags: [algorithm, distribution, fair, resource, sharing]
math: true
permalink: /:title/
hidden: true
---

The following is a rendered version of the *Fairdist Algorithm*, a way to share
and distribute a dynamic set of resources with a dynamic number of peers.

## Prerequisites

 * Let $$c \in \mathbb{R}_{\geq 0}$$ be a total amount of consumed resources.
 * Let $$r \in \mathbb{R}_{\geq 0}$$ be a total amount of reserved resources.
 * Let $$n \in \mathbb{N}_0$$ be a number of peers that consumed resources.
 * Let $$A: \mathbb{N}_0 \to \mathbb{R}_{>0}$$ be a function that computes
   the proportion of $$r$$ a peer can consume, based on the number of peers
   $$n$$ that currently have resources consumed.
 * Let $$G: \mathbb{N}_0 \to \mathbb{R}_{>0}$$ be a function that computes
   the proportion of $$c + r$$ a peer is guaranteed, based on the number of
   peers $$n$$ that currently have resources consumed.

## Definition

The allocator $$A$$ is said to guarantee the limit $$G$$, if there exists a
function $$R: \mathbb{N}_+ \to \mathbb{R}_{>0}$$ so that:

$$r \geq \frac{c}{R(n)}$$

*implies both:*

 1. $$\frac{r}{A(n)} \geq \frac{c+r}{G(n)}$$
 2. $$r - \frac{r}{A(n)} \geq \frac{c + \frac{r}{A(n)}}{R(n+1)}$$

## Lemma 1

To proof an allocator $$A$$ guarantees $$G$$, it is sufficient to show that
$$R$$ fulfils:

$$R(n) \leq \frac{G(n)}{A(n)} - 1$$

and

$$A(n) \geq \frac{1+R(n+1)}{R(n+1)-R(n)}$$

### Proof

First, we prove part 1 of the definition is true, using the first requisite of
this lemma:

$$
\begin{align}
r &\geq_{req} \frac{c}{R(n)}\\[8pt]
R(n) &\geq \frac{c}{r}\\[8pt]
\frac{G(n)}{A(n)} - 1 \geq_{req} R(n) &\geq \frac{c}{r}\\[8pt]
\frac{G(n)}{A(n)} - 1 &\geq \frac{c}{r}\\[8pt]
\frac{r G(n)}{A(n)} - r &\geq c\\[8pt]
\frac{r G(n)}{A(n)} &\geq c+r\\[8pt]
\frac{r}{A(n)} &\geq \frac{c+r}{G(n)}\\[8pt]
\end{align}
$$

Secondly, we prove the second requisite of this lemma implies part 2 of the
definition, under the assumption the requisite of the definition is true:

$$
\begin{align}
A(n) &\geq_{req} \frac{1+R(n+1)}{R(n+1)-R(n)}\\[16pt]
A(n)R(n+1) - A(n)R(n) &\geq 1+R(n+1)\\[16pt]
-A(n)R(n) &\geq 1+R(n+1) - A(n)R(n+1)\\[16pt]
A(n)R(n) &\leq A(n)R(n+1)-R(n+1)-1\\[16pt]
R(n) &\leq R(n+1) - \frac{R(n+1)}{A(n)} - \frac{1}{A(n)}\\[16pt]
\frac{c}{R(n)} &\geq \frac{c}{R(n+1) - \frac{R(n+1)}{A(n)} - \frac{1}{A(n)}}\\[16pt]
r \geq_{req} \frac{c}{R(n)} &\geq \frac{c}{R(n+1) - \frac{R(n+1)}{A(n)} - \frac{1}{A(n)}}\\[16pt]
r &\geq \frac{c}{R(n+1) - \frac{R(n+1)}{A(n)} - \frac{1}{A(n)}}\\[16pt]
rR(n+1) - \frac{rR(n+1)}{A(n)} - \frac{r}{A(n)} &\geq c\\[16pt]
rR(n+1) - \frac{rR(n+1)}{A(n)} &\geq c + \frac{r}{A(n)}\\[16pt]
r - \frac{r}{A(n)} &\geq \frac{c + \frac{r}{A(n)}}{R(n+1)}\\[16pt]
\end{align}
$$

## Theorem

The following allocators each guarantee the specified limit:

$$
\begin{align}
A_1(n) &:= 2\\
G_1(n) &:= 2^{n+1}\\
\\
A_2(n) &:= n+2\\
G_2(n) &:= n^2+3n+2\\
\\
A_3(n) &:= (n+2) \log_2(n+2) + (n+2)\\
G_3(n) &:= \mathcal{O}(n \log_2(n)^2)\\
\end{align}
$$

### Proof

We provide a function $$R$$ for each pair. We then substitute them in _Lemma 1_
and show through equivalence transformations that the assertions are true.

#### Proof 1: Exponential Guarantee

 * _Allocator:_ $$A(n) := 2$$
 * _Guarantee:_ $$G(n) := 2^{n+1}$$

Let $$R(n) := 2^n - 1$$.

_Part 1:_

$$
\begin{align}
R(n) &\leq_{lemma} \frac{G(n)}{A(n)} - 1\\[8pt]
2^n - 1 &\leq \frac{2^{n+1}}{2} - 1\\[8pt]
2^n &= \frac{2^{n+1}}{2}\\[8pt]
2^n &= 2^n\\[8pt]
\end{align}
$$

_Part 2:_

$$
\begin{align}
A(n) &\geq \frac{1+R(n+1)}{R(n+1)-R(n)}\\[8pt]
2 &\geq \frac{1+(2^{n+1} - 1)}{(2^{n+1} - 1)-(2^n - 1)}\\[8pt]
2 &\geq \frac{2^{n+1}}{2^{n+1} - 2^n}\\[8pt]
2 &\geq \frac{2^{n+1}}{2^{n+1}(1 - \frac{1}{2})}\\[8pt]
2 &\geq \frac{1}{1 - \frac{1}{2}}\\[8pt]
2 &\geq 2\\[8pt]
\end{align}
$$

#### Proof 2: Polynomial Guarantee

 * _Allocator:_ $$A(n) := n+2$$
 * _Guarantee:_ $$G(n) := n^2 + 3n + 2$$

Let $$R(n) := n$$.

_Part 1:_

$$
\begin{align}
R(n) &\leq_{lemma} \frac{G(n)}{A(n)} - 1\\[8pt]
n &\leq \frac{n^2 + 3n + 2}{n+2} - 1\\[8pt]
n+1 &\leq \frac{n^2 + 3n + 2}{n+2}\\[8pt]
(n+1)(n+2) &\leq n^2 + 3n + 2\\[8pt]
n^2 + 3n + 2 &\leq n^2 + 3n + 2\\[8pt]
\end{align}
$$

_Part 2:_

$$
\begin{align}
A(n) &\geq \frac{1+R(n+1)}{R(n+1)-R(n)}\\[8pt]
n+2 &\geq \frac{1+(n+1)}{(n+1)-(n)}\\[8pt]
n+2 &\geq \frac{n+2}{n-n+1}\\[8pt]
n+2 &\geq n+2\\[8pt]
\end{align}
$$

#### Proof 3: Quasilinear Guarantee

 * _Allocator:_ $$A(n) := (n+2) \log_2(n+2) + (n+2)$$
 * _Guarantee:_ $$G(n) := \mathcal{O}(n \log_2(n)^2)$$

Let $$R(n) := \log_2(n+1)$$.

_Part 1:_

$$
\begin{align}
R(n) &\leq_{lemma} \frac{G(n)}{A(n)} - 1\\[8pt]
\log_2(n+1) &\leq \frac{\mathcal{O}(n \log_2 (n)^2)}{(n+2) \log_2(n+2) + (n+2)} - 1\\[8pt]
\log_2(n+1) + 1 &\leq \frac{\mathcal{O}(n \log_2 (n)^2)}{(n+2) \log_2(n+2) + (n+2)}\\[8pt]
\log_2(n+1) + 1 &\leq \frac{\mathcal{O}(n \log_2 (n)^2)}{(n+2) (\log_2(n+2) + 1)}\\[8pt]
\log_2(n+1) + 1 \leq \log_2(n+2) + 1 &\leq \frac{\mathcal{O}(n \log_2 (n)^2)}{(n+2) (\log_2(n+2) + 1)}\\[8pt]
(\log_2(n+1) + 1)^2 &\leq \frac{\mathcal{O}(n \log_2 (n)^2)}{(n+2)}\\[8pt]
(n+2) \cdot (\log_2(n+1) + 1)^2 &\leq \mathcal{O}(n \cdot \log_2 (n)^2)\\[8pt]
\end{align}
$$

_Part 2:_

For this part, we rely on the following property:

$$\frac{1}{n+1} \leq \log(n+1) - \log(n) \leq \frac{1}{n}$$

This is true for all logarithms for all $$n \in \mathbb{N}_+$$.

$$
\begin{align}
A(n) &\geq \frac{1+R(n+1)}{R(n+1)-R(n)}\\[8pt]
(n+2) \log_2(n+2) + (n+2) &\geq \frac{1+\log_2((n+1)+1)}{\log_2((n+1)+1) - \log_2(n+1)}\\[8pt]
(n+2) \log_2(n+2) + (n+2) &\geq \frac{1+\log_2(n+2)}{\log_2(n+2) - \log_2(n+1)}\\[8pt]
(n+2) \log_2(n+2) + (n+2) &\geq \frac{1+\log_2(n+2)}{\frac{1}{n+2}}\\[8pt]
(n+2) (\log_2(n+2) + 1) &\geq \frac{1+\log_2(n+2)}{\frac{1}{n+2}}\\[8pt]
(n+2) (\log_2(n+2) + 1) &\geq (n+2) (1+\log_2(n+2))\\[8pt]
\end{align}
$$
